investigations/bedrock2/StateMachineProperties.v
@@ -1,4 +1,6 @@
 Require Import Coq.Lists.List.
+Require Import Coq.Strings.String.
+Require Import bedrock2.ProgramLogic.
 Require Import bedrock2.Semantics.
 Require Import bedrock2.Syntax.
 Require Import bedrock2.WeakestPrecondition.
@@ -18,95 +20,97 @@ Local Open Scope Z_scope.
 Section Proofs.
   Context {width word} {p : StateMachineSemantics.parameters width word}
           {p_ok : parameters.ok p}.
+  Import parameters.
 
   Lemma execution_step action args rets t s s':
     execution t s -> step action s args rets s' ->
     execution ((map.empty, action, args, (map.empty, rets)) :: t) s'.
   Proof. intros; cbn [execution]; eauto. Qed.
 
-  Lemma invert1_execution action args rets t s':
-    execution ((map.empty, action, args, (map.empty, rets)) :: t) s' ->
-    exists s, execution t s /\ step action s args rets s'.
-  Proof. intros; cbn [execution]; eauto. Qed.
-
-  Lemma invert1_step action args rets s s':
-    step action s args rets s' ->
-    (exists r addr val,
-        args = [addr]
-        /\ rets = [val]
-        /\ parameters.reg_addr r = addr
-        /\ parameters.read_step s r val s')
-    \/ (exists r addr val,
-        args = [addr; val]
-        /\ rets = []
-        /\ parameters.reg_addr r = addr
-        /\ parameters.write_step s r val s').
+  Lemma execution_step_read r addr val t s s':
+    execution t s -> reg_addr r = addr -> read_step s r val s' ->
+    execution ((map.empty, READ, [addr], (map.empty, [val])) :: t) s'.
   Proof.
-    inversion 1; subst; [ left | right ];
-      do 3 eexists; ssplit; try reflexivity;
-        assumption.
+    intros. eapply execution_step; [ eassumption | ].
+    cbv [step]. change (READ =? WRITE)%string with false.
+    rewrite String.eqb_refl. eauto.
   Qed.
 
+  Lemma execution_step_write r addr val t s s':
+    execution t s -> reg_addr r = addr -> write_step s r val s' ->
+    execution ((map.empty, WRITE, [addr;val], (map.empty, [])) :: t) s'.
+  Proof.
+    intros. eapply execution_step; [ eassumption | ].
+    cbv [step]. rewrite String.eqb_refl. eauto.
+  Qed.
 
-  Lemma invert1_step_read addr rets s s':
-    step parameters.READ s [addr] rets s' ->
-    (exists r val,
-        parameters.reg_addr r = addr
-        /\ rets = [val]
-        /\ parameters.read_step s r val s').
-  Proof. inversion 1; subst. eexists; eauto. Qed.
-
-  Lemma invert1_step_write addr val rets s s':
-    step parameters.WRITE s [addr; val] rets s' ->
-    (exists r,
-        parameters.reg_addr r = addr
-        /\ rets = []
-        /\ parameters.write_step s r val s').
-  Proof. inversion 1; subst. eexists; eauto. Qed.
-
-  Lemma interact_mmio call action binds arges t m l
-        (post : trace -> mem -> locals -> Prop) (args : list Semantics.word) :
-    dexprs m l arges args ->
-    (forall s' (rets : list Semantics.word),
-        execution ((map.empty, action, args, (map.empty, rets)) :: t) s' ->
-        (exists l0 : locals,
-            map.putmany_of_list_zip binds rets l = Some l0 /\
-            post ((map.empty, action, args, (map.empty, rets)) :: t) m l0)) ->
-    cmd call (cmd.interact binds action arges) t m l post.
+  Lemma interact_read r call bind addre t m l (post : trace -> mem -> locals -> Prop) addr :
+    dexprs m l [addre] [addr] ->
+    reg_addr r = addr ->
+    (exists s s' val, execution t s /\ read_step s r val s') ->
+    (forall s s' val,
+        execution t s ->
+        read_step s r val s' ->
+        (* implied by other preconditions but convenient to have separately *)
+        execution ((map.empty, READ, [addr], (map.empty, [val])) :: t) s' ->
+        post ((map.empty, READ, [addr], (map.empty, [val])) :: t)
+             m (map.put l bind val)) ->
+    cmd call (cmd.interact [bind] READ [addre]) t m l post.
   Proof.
     intros. eapply interact_nomem; [ eassumption | ].
     cbn [Semantics.ext_spec semantics_parameters].
-    cbv [ext_spec]. split; [reflexivity | ].
-    intros. split; [ reflexivity | ].
-    cbn [execution] in *; destruct_products.
-    eauto.
+    cbv [ext_spec]. change (READ =? WRITE)%string with false.
+    rewrite String.eqb_refl.
+    do 2 eexists; ssplit; [ reflexivity || eassumption .. | ].
+    intros; ssplit; [ reflexivity | ].
+    repeat straightline. eauto using execution_step_read.
+  Qed.
+
+  Lemma interact_write r call addre vale t m l
+        (post : trace -> mem -> locals -> Prop)  addr val :
+    dexprs m l [addre;vale] [addr;val] ->
+    reg_addr r = addr ->
+    (exists s s', execution t s /\ write_step s r val s') ->
+    (forall s s',
+        execution t s ->
+        write_step s r val s' ->
+        (* implied by other preconditions but convenient to have separately *)
+        execution ((map.empty, WRITE, [addr;val], (map.empty, [])) :: t) s' ->
+        post ((map.empty, WRITE, [addr;val], (map.empty, [])) :: t) m l) ->
+    cmd call (cmd.interact [] WRITE [addre; vale]) t m l post.
+  Proof.
+    intros. eapply interact_nomem; [ eassumption | ].
+    cbn [Semantics.ext_spec semantics_parameters].
+    cbv [ext_spec]. rewrite String.eqb_refl.
+    do 3 eexists; ssplit; [ reflexivity || eassumption .. | ].
+    intros; ssplit; [ reflexivity | ].
+    repeat straightline. eauto using execution_step_write.
   Qed.
 End Proofs.
 
 (**** Tactics for state machine proofs ****)
 
-Ltac invert_step :=
-  lazymatch goal with
-  | H : step _ _ _ _ _ |- _ =>
-    first [ apply @invert1_step_read in H; destruct H as [? [? [? [? ?]]]]
-          | apply @invert1_step_write in H; destruct H as [? [? [? ?]]]
-          | inversion H; clear H ]; subst;
-    repeat lazymatch goal with
-           | H : _ :: _ = _ :: _ |- _ => inversion H; clear H; subst end
-  end.
+Ltac solve_dexprs :=
+  fail "Redefine the solve_dexprs tactic, and the new definition will be applied
+  to the dexprs side condition of interact_read and interact_write!".
 
-(* shorthand for applying [interact_mmio] and then doing some simplification
-   afterwards; takes a tactic argument which is run on the [dexprs] side
-   condition generated by interact_mmio *)
-Ltac interaction tac :=
-  (* get trace *)
-  let t := lazymatch goal with
-           | |- cmd _ (cmd.interact _ _ _) ?t _ _ _ => t end in
-  eapply interact_mmio; [ tac | ]; intros;
-  lazymatch goal with
-  | H : execution (_ :: t) _ |- _ =>
-    pose proof H; apply invert1_execution in H; destruct H as [? [? ?]]
-  end; invert_step.
+Ltac interact_read_reg reg :=
+  eapply (interact_read reg);
+  [ solve_dexprs
+  | reflexivity
+  | do 3 eexists; split; [ eassumption | ];
+    cbv [parameters.read_step]; eauto
+  | ];
+  repeat straightline.
+
+Ltac interact_write_reg reg :=
+  eapply (interact_write reg);
+  [ solve_dexprs
+  | reflexivity
+  | do 2 eexists; ssplit; [ eassumption | ];
+    cbv [parameters.write_step]; eauto
+  | ];
+  repeat straightline.
 
 (* Remove [execution] hypotheses that are superceded by later ones; improves
    proof performance *)
